sketch ingredients needed to connect a bw simulation from kami impl to riscv spec with a post-condition style program logic & compiler correctness proof

processor/src/Test.v
@@ -1,5 +1,6 @@
 Require Import Coq.ZArith.ZArith.
 Require Import Coq.micromega.Lia.
+Require Import Coq.Lists.List. Import ListNotations.
 Require Import riscv.Decode.
 Require Import riscv.Encode.
 Require Import coqutil.Word.LittleEndian.
@@ -17,15 +18,19 @@ Require Import riscv.proofs.DecodeEncode.
 Require Import riscv.Run.
 Require Import riscv.MkMachineWidth.
 Require Import riscv.util.Monads.
-
+Require Import riscv.runsToNonDet.
+Require Import coqutil.Datatypes.PropSet.
+Require Import riscv.MMIOTrace.
 
 Local Open Scope Z_scope.
 
 Section Equiv.
 
   (* TODO not sure if we want to use ` or rather a parameter record *)
-  Context `{Pr: Primitives}.
+  Context {M: Type -> Type}.
+  Context `{Pr: Primitives MMIOAction M}.
   Context {RVS: RiscvState M word}.
+  Notation RiscvMachine := (RiscvMachine Register MMIOAction).
 
   Definition NOP: w32 := LittleEndian.split 4 (encode (IInstruction Nop)).
 
@@ -37,7 +42,7 @@ Section Equiv.
   Definition fakeStep: FakeProcessor -> FakeProcessor :=
     fun '(Build_FakeProcessor c nc) => Build_FakeProcessor nc (word.add nc (word.of_Z 4)).
 
-  Definition from_Fake(f: FakeProcessor): RiscvMachine Register Action := {|
+  Definition from_Fake(f: FakeProcessor): RiscvMachine := {|
     getRegs := map.empty;
     getPc := f.(counter);
     getNextPc := f.(nextCounter);
@@ -45,7 +50,7 @@ Section Equiv.
     getLog := nil;
   |}.
 
-  Definition to_Fake(m: RiscvMachine Register Action): FakeProcessor := {|
+  Definition to_Fake(m: RiscvMachine): FakeProcessor := {|
     counter := m.(getPc);
     nextCounter := m.(getNextPc);
   |}.
@@ -65,8 +70,8 @@ Section Equiv.
 
   Hypothesis assume_no_MMIO: forall mach addr post, ~ nonmem_loadWord_sat mach addr post.
 
-  Lemma simulate_step_fw: forall (initial: RiscvMachine Register Action)
-                                 (post: RiscvMachine Register Action -> Prop),
+  Lemma simulate_step_fw: forall (initial: RiscvMachine)
+                                 (post: RiscvMachine -> Prop),
       (* begin additional hypotheses which should be deleted in a real proof *)
       Memory.loadWord initial.(getMem) initial.(getPc) = Some NOP ->
       (forall machine1 machine2,
@@ -121,30 +126,158 @@ Section Equiv.
       Memory.loadWord (Memory.unchecked_store_bytes 4 m addr w) addr = Some w.
   Admitted. (* TODO once we have a good map solver and word solver, this should be easy *)
 
-  (* list is kind of redundant (already in RiscvMachine.(getLog)))
-     and should at most contain one event *)
-  Inductive riscvStep: RiscvMachine Register Action -> RiscvMachine Register Action -> list (LogItem Action) -> Prop :=
-  | foo: forall initialL finalL t post,
-      mcomp_sat (run1 iset) initialL post ->
-      post tt finalL ->
-      riscvStep initialL finalL t.
+  Lemma to_Fake_from_Fake: forall (m: FakeProcessor),
+      to_Fake (from_Fake m) = m.
+  Proof.
+    intros. destruct m. reflexivity.
+  Qed.
 
+  Lemma from_Fake_to_Fake: forall (m: RiscvMachine),
+      from_Fake (to_Fake m) = m.
+  Proof.
+    intros. destruct m. unfold to_Fake, from_Fake. simpl.
+    (* Doesn't hold for the fake processor! *)
+  Admitted.
+
+  (* common event between riscv-coq and Kami *)
   Inductive Event: Type :=
   | MMInputEvent(addr v: word)
   | MMOutputEvent(addr v: word).
 
-  Definition riscvTrace_to_common: list (LogItem Action) -> list Event. Admitted.
-  Definition commonTrace_to_riscv: list Event -> list (LogItem Action). Admitted.
+  Definition riscvEvent_to_common(e: LogItem MMIOAction): Event :=
+    match e with
+    | ((m1, MMInput, [addr]), (m2, [v])) => MMInputEvent addr v
+    | ((m1, MMOutput, [addr; v]), (m2, [])) => MMOutputEvent addr v
+    | _ => MMOutputEvent (word.of_Z 0) (word.of_Z 0) (* TODO what to do in error case? *)
+    end.
+
+  Definition riscvTrace_to_common: list (LogItem MMIOAction) -> list Event :=
+    List.map riscvEvent_to_common.
+
+  (* TODO!! this direction cannot be defined because it misses information such as the memory *)
+  Definition commonEvent_to_riscv: Event -> LogItem MMIOAction. Admitted.
+  Definition commonTrace_to_riscv: list Event -> list (LogItem MMIOAction) :=
+    List.map commonEvent_to_riscv.
+
+  (* redefine mcomp_sat to simplify for the case where no answer is returned *)
+  Definition mcomp_sat_unit(m: M unit)(initialL: RiscvMachine)(post: RiscvMachine -> Prop): Prop :=
+    mcomp_sat m initialL (fun (_: unit) => post).
+
+  (* list is kind of redundant (already in RiscvMachine.(getLog)))
+     and should at most contain one event,
+     but we still want it to appear in the signature so that we can easily talk about prefixes,
+     and to match Kami's step signature *)
+  Inductive riscvStep: RiscvMachine -> RiscvMachine -> list (LogItem MMIOAction) -> Prop :=
+  | mk_riscvStep: forall initialL finalL t post,
+      mcomp_sat_unit (run1 iset) initialL post ->
+      post finalL ->
+      finalL.(getLog) = t ++ initialL.(getLog) ->
+      riscvStep initialL finalL t.
+
+  Inductive star{S E: Type}(R: S -> S -> list E -> Prop): S -> S -> list E -> Prop :=
+  | star_refl: forall (x: S),
+      star R x x nil
+  | star_step: forall (x y z: S) (t1 t2: list E),
+      star R x y t1 ->
+      R y z t2 ->
+      star R x z (t2 ++ t1).
+
+  (* temporal prefixes, new events are added in front of the head of the list *)
+  Definition prefixes{E: Type}(traces: list E -> Prop): list E -> Prop :=
+    fun prefix => exists rest, traces (rest ++ prefix).
+
+  Definition riscvTraces(initial: RiscvMachine): list Event -> Prop :=
+    fun t => exists final t', star riscvStep initial final t' /\ riscvTrace_to_common t' = t.
+
+  Definition post_to_traces(post: RiscvMachine -> Prop): list Event -> Prop :=
+    fun t => exists final, post final /\ t = riscvTrace_to_common final.(getLog).
+
+  Definition runsTo: RiscvMachine -> (RiscvMachine -> Prop) -> Prop :=
+    runsTo (mcomp_sat_unit (run1 iset)).
+
+  Lemma bridge(init: RiscvMachine)(post: RiscvMachine -> Prop):
+    runsTo init post ->
+    subset (riscvTraces init) (prefixes (post_to_traces post)).
+  Admitted.
 
   Axiom fakestep: FakeProcessor -> FakeProcessor -> list Event -> Prop.
 
-  Lemma simulate: forall (m m': FakeProcessor) t,
+  Lemma simulate_bw_step: forall (m m': FakeProcessor) (t: list Event),
       fakestep m m' t ->
       riscvStep (from_Fake m) (from_Fake m') (commonTrace_to_riscv t).
   Proof.
     intros.
     econstructor.
-  Abort.
+  Admitted.
+
+  Section Lift.
+    Context {S1 S2 E1 E2: Type}.
+    Context (step1: S1 -> S1 -> list E1 -> Prop).
+    Context (step2: S2 -> S2 -> list E2 -> Prop).
+    Context (convert_state: S1 -> S2) (convert_event: E1 -> E2).
+    Hypothesis sim: forall s1 s1' t1,
+        step1 s1 s1' t1 ->
+        step2 (convert_state s1) (convert_state s1') (List.map convert_event t1).
+
+    Lemma lift_star_simulation: forall s1 s1' t1,
+        star step1 s1 s1' t1 ->
+        star step2 (convert_state s1) (convert_state s1') (List.map convert_event t1).
+    Proof.
+      induction 1; [apply star_refl|].
+      rewrite map_app.
+      eapply star_step.
+      - apply IHstar.
+      - eapply sim. assumption.
+    Qed.
+  End Lift.
+
+  (* TODO the "from_Fake" direction doesn't really work *)
+  Lemma simulate_bw_star: forall (m m': FakeProcessor) (t: list Event),
+      star fakestep m m' t ->
+      star riscvStep (from_Fake m) (from_Fake m') (commonTrace_to_riscv t).
+  Proof.
+    apply lift_star_simulation. apply simulate_bw_step.
+  Qed.
+
+  Definition fakeTraces(init: FakeProcessor): list Event -> Prop :=
+    fun t => exists final, star fakestep init final t.
+
+  Lemma connection: forall (m: FakeProcessor),
+      subset (fakeTraces m) (riscvTraces (from_Fake m)).
+  Proof.
+    intros m t H. unfold fakeTraces, riscvTraces in *.
+    destruct H as [m' H].
+    apply simulate_bw_star in H.
+    do 2 eexists; split; [eassumption|].
+    (* TODO trace conversion does not really commute *)
+  Admitted.
+
+  (* assume this first converts the FakeProcessor from SpecProcessor to ImplProcessor state,
+     and also converts from Kami trace to common trace *)
+  Definition kamiImplTraces(init: FakeProcessor): list Event -> Prop. Admitted.
+
+  Axiom kamiImplSoundness: forall (init: FakeProcessor),
+      subset (kamiImplTraces init) (fakeTraces init).
+
+  Lemma subset_trans{A: Type}(s1 s2 s3: A -> Prop):
+    subset s1 s2 ->
+    subset s2 s3 ->
+    subset s1 s3.
+  Proof. unfold subset. auto. Qed.
+
+  Lemma subset_refl{A: Type}(s: A -> Prop): subset s s. Proof. unfold subset. auto. Qed.
+
+  Lemma impl_to_end_of_compiler(init: RiscvMachine)(post: RiscvMachine -> Prop):
+      runsTo init post -> (* <-- will be proved by bedrock2 program logic & compiler *)
+      subset (kamiImplTraces (to_Fake init)) (prefixes (post_to_traces post)).
+  Proof.
+    intro H.
+    eapply subset_trans; [apply kamiImplSoundness|].
+    eapply subset_trans; [|apply bridge; eassumption].
+    eapply subset_trans; [apply connection|].
+    rewrite from_Fake_to_Fake. (* <-- TODO doesn't hold! *)
+    apply subset_refl.
+  Qed.
 
   Lemma simulate_step_bw: forall (m m': FakeProcessor),
       fakeStep m = m' ->
@@ -184,12 +317,6 @@ Section Equiv.
     apply spec_step. simpl. reflexivity.
   Qed.
 
-  Lemma to_Fake_from_Fake: forall (m: FakeProcessor),
-      to_Fake (from_Fake m) = m.
-  Proof.
-    intros. destruct m. reflexivity.
-  Qed.
-
   Lemma step_equiv_too_weak: forall (m m': FakeProcessor),
       fakeStep m = m' <->
       mcomp_sat (run1 iset) (from_Fake m) (fun _ final => to_Fake final = m').
@@ -206,15 +333,8 @@ Section Equiv.
       + assumption.
   Qed.
 
-  Lemma from_Fake_to_Fake: forall (m: RiscvMachine Register Action),
-      from_Fake (to_Fake m) = m.
-  Proof.
-    intros. destruct m. unfold to_Fake, from_Fake. simpl.
-    (* Doesn't hold for the fake processor! *)
-  Admitted.
-
   Lemma weaken_mcomp_sat:
-    forall A m initial (post1 post2: A -> RiscvMachine Register Action -> Prop),
+    forall A m initial (post1 post2: A -> RiscvMachine -> Prop),
       mcomp_sat m initial post1 ->
       (forall (a: A) final, post1 a final -> post2 a final) ->
       mcomp_sat m initial post2.
@@ -230,8 +350,8 @@ Section Equiv.
     assumption.
   Qed.
 
-  Lemma step_equiv: forall (initial: RiscvMachine Register Action)
-                           (post: RiscvMachine Register Action -> Prop),
+  Lemma step_equiv: forall (initial: RiscvMachine)
+                           (post: RiscvMachine -> Prop),
       post (from_Fake (fakeStep (to_Fake initial))) <->
       mcomp_sat (run1 iset) initial (fun _ => post).
   Proof.
